example: `clear.cst`

examples/clear/clear.c
@@ -1,0 +1,205 @@
+#include "vst_ide.h"
+
+void clear(void *to, int len)
+/*@
+With
+  (n : Z)
+Require
+  n >= 0 &&
+  len == n &&
+  store_undef_array(undef_store_char, to, n)
+Ensure
+  store_array(store_char, to, n, Zrepeat(0, n))
+*/
+{
+    /*@ Assert
+      n >= 0 &&
+      len@pre == n &&
+      data_at(&len, int, len@pre) *
+      data_at(&to, void*, to@pre) *
+      store_undef_array(undef_store_char, to@pre, n)
+    */
+    // clear_entail_wit_2
+    /*@ Assert
+      n >= 0 &&
+      data_at(&len, int, n) *
+      data_at(&to, void*, to@pre) *
+      store_undef_array(undef_store_char, to@pre, n)
+    */
+    int i = 0;
+    /*@ Assert
+      n >= 0 &&
+      data_at(&i, int, 0) *
+      data_at(&len, int, n) *
+      data_at(&to, void*, to@pre) *
+      store_undef_array(undef_store_char, to@pre, n)
+    */
+
+    // clear_which_implies_wit_1
+    /*@
+      emp
+      which implies
+      store_array(store_char, to@pre, 0, Zrepeat(0, 0))
+    */
+
+    /*@ Assert
+      n >= 0 &&
+      data_at(&i, int, 0) *
+      data_at(&len, int, n) *
+      data_at(&to, void*, to@pre) *
+      store_array(store_char, to@pre, 0, Zrepeat(0, 0)) *
+      store_undef_array(undef_store_char, to@pre, n)
+    */
+    // clear_entail_wit_5
+    /*@ Assert
+      0 <= 0 && 0 <= n &&
+      n >= 0 &&
+      data_at(&i, int, 0) *
+      data_at(&len, int, n) *
+      data_at(&to, void*, to@pre) *
+      store_array(store_char, to@pre, 0, Zrepeat(0, 0)) *
+      store_undef_array(undef_store_char, to@pre + 0 * sizeof(char), n - 0)
+    */
+
+    /*@ Assert Inv
+      exists i_v,
+      0 <= i_v && i_v <= n &&
+      n >= 0 &&
+      data_at(&i, int, i_v) *
+      data_at(&len, int, n) *
+      data_at(&to, void*, to@pre) *
+      store_array(store_char, to@pre, i_v, Zrepeat(0, i_v)) *
+      store_undef_array(undef_store_char, to@pre + i_v * sizeof(char), n - i_v)
+    */
+    while (i < len)
+    {
+        /*@ Assert
+          exists i_v,
+          i_v < n &&
+          0 <= i_v && i_v <= n &&
+          n >= 0 &&
+          data_at(&i, int, i_v) *
+          data_at(&len, int, n) *
+          data_at(&to, void*, to@pre) *
+          store_array(store_char, to@pre, i_v, Zrepeat(0, i_v)) *
+          store_undef_array(undef_store_char, to@pre + i_v * sizeof(char), n - i_v)
+        */
+
+        // clear_which_implies_wit_2
+        /*@
+          exists i_v,
+          i_v < n &&
+          n >= 0 &&
+          store_undef_array(undef_store_char, to@pre + i_v * sizeof(char), n - i_v)
+          which implies
+          undef_data_at(to@pre + i_v * sizeof(char), char) *
+          store_undef_array(undef_store_char, to@pre + (i_v + 1) * sizeof(char), n - (i_v + 1))
+        */
+
+        /*@ Assert
+          exists i_v,
+          i_v < n &&
+          0 <= i_v && i_v <= n &&
+          n >= 0 &&
+          data_at(&i, int, i_v) *
+          data_at(&len, int, n) *
+          data_at(&to, void*, to@pre) *
+          store_array(store_char, to@pre, i_v, Zrepeat(0, i_v)) *
+          undef_data_at(to@pre + i_v * sizeof(char), char) *
+          store_undef_array(undef_store_char, to@pre + (i_v + 1) * sizeof(char), n - (i_v + 1))
+        */
+        *((char *)to + i) = (char) 0;
+        /*@ Assert
+          exists i_v,
+          i_v < n &&
+          0 <= i_v && i_v <= n &&
+          n >= 0 &&
+          data_at(&i, int, i_v) *
+          data_at(&len, int, n) *
+          data_at(&to, void*, to@pre) *
+          store_array(store_char, to@pre, i_v, Zrepeat(0, i_v)) *
+          data_at(to@pre + i_v * sizeof(char), char, 0) *
+          store_undef_array(undef_store_char, to@pre + (i_v + 1) * sizeof(char), n - (i_v + 1))
+        */
+        i = i + 1;
+        /*@ Assert
+          exists i_v,
+          i_v < n &&
+          0 <= i_v && i_v <= n &&
+          n >= 0 &&
+          data_at(&i, int, i_v + 1) *
+          data_at(&len, int, n) *
+          data_at(&to, void*, to@pre) *
+          store_array(store_char, to@pre, i_v, Zrepeat(0, i_v)) *
+          data_at(to@pre + i_v * sizeof(char), char, 0) *
+          store_undef_array(undef_store_char, to@pre + (i_v + 1) * sizeof(char), n - (i_v + 1))
+        */
+
+        // clear_which_implies_wit_3
+        /*@
+          exists i_v,
+          store_array(store_char, to@pre, i_v, Zrepeat(0, i_v)) *
+          data_at(to@pre + i_v * sizeof(char), char, 0)
+          which implies
+          store_array(store_char, to@pre, i_v + 1, Zrepeat(0, i_v + 1))
+        */
+
+        /*@ Assert
+          exists i_v,
+          i_v < n &&
+          0 <= i_v && i_v <= n &&
+          n >= 0 &&
+          data_at(&i, int, i_v + 1) *
+          data_at(&len, int, n) *
+          data_at(&to, void*, to@pre) *
+          store_array(store_char, to@pre, i_v + 1, Zrepeat(0, i_v + 1)) *
+          store_undef_array(undef_store_char, to@pre + (i_v + 1) * sizeof(char), n - (i_v + 1))
+        */
+        // clear_entail_wit_12
+        /*@ Assert
+          exists i_v,
+          0 <= i_v + 1 && i_v + 1 <= n &&
+          n >= 0 &&
+          data_at(&i, int, i_v + 1) *
+          data_at(&len, int, n) *
+          data_at(&to, void*, to@pre) *
+          store_array(store_char, to@pre, i_v + 1, Zrepeat(0, i_v + 1)) *
+          store_undef_array(undef_store_char, to@pre + (i_v + 1) * sizeof(char), n - (i_v + 1))
+        */
+    }
+    /*@ Assert
+      exists i_v,
+      i_v >= n &&
+      0 <= i_v && i_v <= n &&
+      n >= 0 &&
+      data_at(&i, int, i_v) *
+      data_at(&len, int, n) *
+      data_at(&to, void*, to@pre) *
+      store_array(store_char, to@pre, i_v, Zrepeat(0, i_v)) *
+      store_undef_array(undef_store_char, to@pre + i_v * sizeof(char), n - i_v)
+    */
+    // clear_entail_wit_15
+    /*@ Assert
+      n >= 0 &&
+      data_at(&i, int, n) *
+      data_at(&len, int, n) *
+      data_at(&to, void*, to@pre) *
+      store_array(store_char, to@pre, n, Zrepeat(0, n)) *
+      store_undef_array(undef_store_char, to@pre + n * sizeof(char), n - n)
+    */
+
+    // clear_which_implies_wit_4
+    /*@
+      store_undef_array(undef_store_char, to@pre + n * sizeof(char), n - n)
+      which implies
+      emp
+    */
+
+    /*@ Assert
+      n >= 0 &&
+      data_at(&i, int, n) *
+      data_at(&len, int, n) *
+      data_at(&to, void*, to@pre) *
+      store_array(store_char, to@pre, n, Zrepeat(0, n))
+    */
+}
