lcf_server/hol-light-helper/helpers.ml
@@ -1,5 +1,3 @@
-needs "simp.ml";;
-
 let topeval code =
   let as_buf = Lexing.from_string code in
   let parsed = !Toploop.parse_toplevel_phrase as_buf in
@@ -126,3 +124,34 @@ let ssubst tm1 tm2 tm = subst[tm1, tm2] tm;;
 let apply_conv conv tm = conv tm;;
 
 let hypth th = hd (hyp th);;
+let equals_term t1 t2 = t1 = t2;;
+
+let ARITH_RULE_SAFETY =
+  let init_conv =
+    NUM_SIMPLIFY_CONV THENC
+    GEN_REWRITE_CONV DEPTH_CONV [ADD1] THENC
+    PROP_ATOM_CONV (BINOP_CONV NUM_NORMALIZE_CONV) THENC
+    PRENEX_CONV THENC
+    (GEN_REWRITE_CONV TOP_SWEEP_CONV o map GSYM)
+      [INT_OF_NUM_EQ; INT_OF_NUM_LE; INT_OF_NUM_LT; INT_OF_NUM_GE;
+       INT_OF_NUM_GT; INT_OF_NUM_ADD; SPEC `NUMERAL k` INT_OF_NUM_MUL;
+       INT_OF_NUM_MAX; INT_OF_NUM_MIN]
+  and is_numimage t =
+    match t with
+      Comb(Const("int_of_num",_),n) when not(is_numeral n) -> true
+    | _ -> false in
+  fun tm ->
+    try
+      let th1 = init_conv tm in
+      let tm1 = rand(concl th1) in
+      let avs,bod = strip_forall tm1 in
+      let nim = setify(find_terms is_numimage bod) in
+      let gvs = map (genvar o type_of) nim in
+      let pths = map (fun v -> SPEC (rand v) INT_POS) nim in
+      let ibod = itlist (curry mk_imp o concl) pths bod in
+      let gbod = subst (zip gvs nim) ibod in
+      let th2 = INST (zip nim gvs) (INT_ARITH gbod) in
+      let th3 = GENL avs (rev_itlist (C MP) pths th2) in
+      EQ_MP (SYM th1) th3
+    with Failure _ -> TRUTH 
+;;
