lcf_server/includes/proof-conv.h
@@ -1,6 +1,13 @@
 #include <proof-user.h>
 
+thm trans_list(thm thl[]);
+thm rewrite_list(thm thl[], term tm);
+thm rewrite_rule_list(thm thl[], thm th);
+thm hentail_trans_list(thm thl[]);
+
+term normalize(term septerm);
 thm sep_normalize(term septerm);
+thm sep_normalize_rule(thm entail);
 thm sep_lift(term lft, term septerm);
 thm sep_cancel(term lft, term septerm);
 thm which_implies(term state, thm trans);
