lcf_server/proof-user/proof-conv.c
@@ -2,26 +2,7 @@
 #include <string.h>
 #include <stdio.h>
 
-bool equal(term tm1, term tm2) {
-  return !strcmp(string_of_term(tm1), string_of_term(tm2));
-}
-
-thm sep_normalize_(term septerm) {
-  if (is_binop(parse_term("hsep"), septerm)) {
-    term l = fst_binop(parse_term("hsep"), septerm), r = snd_binop(parse_term("hsep"), septerm);
-    if (is_comb(r) && equal(fst_comb(r), parse_term("hfact"))) {
-      thm th1 = once_rewrite(get_theorem("hsep_hfact_comm"), septerm);
-      septerm = snd_comb(concl(th1));
-      r = snd_comb(septerm);
-      thm th2 = once_rewrite(sep_normalize_(r), septerm);
-      return trans(th1, th2);
-    } else {
-      return once_rewrite(sep_normalize_(l), septerm);
-    } 
-  } else {
-    return refl(septerm);
-  }
-}
+#define N 100
 
 /// Suppose `thl` end with `NULL`.
 thm rewrite_list(thm thl[], term tm) {
@@ -29,7 +10,7 @@ thm rewrite_list(thm thl[], term tm) {
   thm result = rewrite(thl[0], tm);
   for (int i = 1; ; ++i) {
     if (thl[i] == NULL) break;
-    result = trans(result, rewrite(thl[i], snd_comb(concl(result))));
+    result = trans(result, rewrite(thl[i], snd_comb(conclusion(result))));
   }
   return result;
 }
@@ -45,6 +26,54 @@ thm trans_list(thm thl[]) {
   return result;
 }
 
+/// Suppose `thl` end with `NULL`.
+thm rewrite_rule_list(thm thl[], thm th) {
+  if (thl[0] == NULL) return NULL;
+  thm result = rewrite_rule(thl[0], th);
+  for (int i = 1; ; ++i) {
+    if (thl[i] == NULL) break;
+    result = rewrite_rule(thl[i], result);
+  }
+  return result;
+}
+
+thm hentail_trans_list(thm thl[]) {
+  thm hentail_trans = get_theorem("hentail_trans");
+  thm result = thl[0];
+
+  for (int i = 1; ; ++i) {
+    if (thl[i] == NULL) break;
+    result = mp(mp(hentail_trans, result), thl[i]);
+  }
+  return result;
+}
+
+
+bool has_typ(thm th) {
+  return !equals_thm(new_axiom(conclusion(th)), th);
+}
+
+term normalize(term septerm) {
+  return consequent(conclusion(sep_normalize(septerm)));
+}
+
+thm sep_normalize_(term septerm) {
+  if (is_binop(parse_term("hsep"), septerm)) {
+    term l = fst_binop(parse_term("hsep"), septerm), r = snd_binop(parse_term("hsep"), septerm);
+    if (is_comb(r) && equals_term(fst_comb(r), parse_term("hfact"))) {
+      thm th1 = once_rewrite(get_theorem("hsep_hfact_comm"), septerm);
+      septerm = snd_comb(conclusion(th1));
+      r = snd_comb(septerm);
+      thm th2 = once_rewrite(sep_normalize_(r), septerm);
+      return trans(th1, th2);
+    } else {
+      return once_rewrite(sep_normalize_(l), septerm);
+    } 
+  } else {
+    return refl(septerm);
+  }
+}
+
 thm sep_normalize(term septerm) {
   thm th1 = rewrite_list( 
     (thm[]) { get_theorem("hand_assoc"), 
@@ -54,15 +83,15 @@ thm sep_normalize(term septerm) {
               get_theorem("hsep_hemp_left"),
               get_theorem("hsep_hemp_right"),
               NULL }, septerm);
-  septerm = snd_comb(concl(th1));
+  septerm = consequent(conclusion(th1));
   thm th2 = sep_normalize_(septerm);
-  septerm = snd_comb(concl(th2));
+  septerm = consequent(conclusion(th2));
   thm th3 = rewrite(get_theorem("hsep_assoc"), septerm);
   return trans_list((thm[]){th1, th2, th3, NULL});
 }
 
 thm sep_normalize_rule(thm th) {
-  term septerm = concl(th);
+  term septerm = conclusion(th);
   if (is_binop(parse_term("hentail"), septerm)) {
     term l = fst_binop(parse_term("hentail"), septerm), r = snd_binop(parse_term("hentail"), septerm);
     th = rewrite_rule(sep_normalize(l), th);
@@ -77,13 +106,13 @@ thm sep_lift_(term lft, term septerm) {
   thm lem1 = spec(lft, get_theorem("hsep_comm_left_part"));
 
   if (is_binop(parse_term("hsep"), septerm)) {
-    term l = snd_comb(fst_comb(septerm)), r = snd_comb(septerm);
-    if (equal(l, lft)) {
+    term l = fst_binop(parse_term("hsep"), septerm), r = snd_binop(parse_term("hsep"), septerm);
+    if (equals_term(l, lft)) {
       return once_rewrite(lem1, septerm);
     } else {
       if (is_binop(parse_term("hsep"), r)) {
         thm th1 = once_rewrite(sep_lift_(lft, r), septerm);
-        septerm = snd_comb(concl(th1));
+        septerm = consequent(conclusion(th1));
         thm th2 = once_rewrite(lem1, septerm);
         return trans(th1, th2);
       } else {
@@ -97,11 +126,11 @@ thm sep_lift_(term lft, term septerm) {
 
 thm sep_lift(term lft, term septerm) {
   if (is_binop(parse_term("hsep"), lft)) {
-    term l = snd_comb(fst_comb(lft)), r = snd_comb(lft);
+    term l = fst_binop(parse_term("hsep"), lft), r = snd_binop(parse_term("hsep"), lft);
     thm th1 = sep_lift(r, septerm);
-    septerm = snd_comb(concl(th1));
+    septerm = consequent(conclusion(th1));
     thm th2 = sep_lift_(l, septerm);
-    septerm = snd_comb(concl(th2));
+    septerm = consequent(conclusion(th2));
     thm th3 = once_rewrite(symm(get_theorem("hsep_assoc")), septerm);
     return trans_list((thm[]){th1, th2, th3, NULL});
   } else {
@@ -113,8 +142,8 @@ thm sep_cancel(term lft, term septerm) {
   if (is_binop(parse_term("hsep"), lft)) {
     term l = fst_binop(parse_term("hsep"), lft);
     term r = snd_binop(parse_term("hsep"), lft);
-    thm th1 = sep_lift_(l, septerm);
-    septerm = snd_comb(concl(th1));
+    thm th1 = once_rewrite(sep_lift_(l, septerm), septerm);
+    septerm = consequent(conclusion(th1));
     thm th2 = once_rewrite(sep_cancel(r, snd_comb(septerm)), septerm);
     return trans(th1, th2);
   } else {
@@ -122,16 +151,14 @@ thm sep_cancel(term lft, term septerm) {
   }
 }
 
-#define N 100
-term exists_list[N];
-int exists_count = 0;
-#undef N 
-
 thm which_implies(term state, thm th) {
-  /// `state` is in the form of `hexists x1..xn. Q1 ** ... ** Qn.
-  /// `th` is in the form of `P1 ==> (.. (Pn ==> (Q1 ** ... ** Qn |-- R1 ** ... ** Rn)))`.
+  /// `state` is in the form of `hexists x1..xn. Q1 ** ... ** Qx.
+  /// `th` is in the form of `P1 ==> (.. (Pn ==> (Q1 ** ... ** Qm |-- R1 ** ... ** Rs)))`.
+  /// suppose pre- and post-condition of `th` are not `emp`.
 
   // Destruct `hexists` and record the binders in `exists_list`.
+  term exists_list[N];
+  int exists_count = 0;
   while (is_binder("hexists", state)) {
     exists_list[++exists_count] = binder_var("hexists", state);
     state = binder_body("hexists", state);
@@ -143,35 +170,36 @@ thm which_implies(term state, thm th) {
     figure this out by check if the return value is `NULL`, and (temporarily) ignore 
     the error information raised by OCaml (actually Rust). 
   */
-  while (1) {
+  while (is_binop(parse_term("==>"), conclusion(th))) {
     thm tmp = undisch(th);
     if (tmp == NULL) break;
     th = undisch(th);
   }
-  while (1) {
+  while (has_typ(th)) {
     term hyp = hypth(th);
     if (hyp == NULL) break;
     th = disch(th, hyp);
-    th = mp(get_theorem("hfact_elim"), th);
+    th = mp(get_theorem("hfact_elim_dup"), th);
   }
   th = sep_normalize_rule(th);
-  term th_pre = fst_binop(parse_term("hentail"), concl(th));
-  term th_post = snd_binop(parse_term("hentail"), concl(th));
-  
+  term th_pre = fst_binop(parse_term("hentail"), conclusion(th));
+  term th_post = snd_binop(parse_term("hentail"), conclusion(th));
   /*  Apply `trans` theorem .
     First normalize `state` to a form `(trans_pre) * (other)`. Then apply `hsep_cancel_right` 
     rule to get a theorem `(trans_pre) * (other) |-- (trans_post) * (other)`. Finally return 
     the normalized post condition of this entailment. 
   */ 
-  term old_state = state;
   thm th1 = sep_normalize(state);
-  state = snd_comb(concl(th1));
+  state = consequent(conclusion(th1));
+  term old_state = state;
   thm th2 = sep_lift(th_pre, state);
-  state = snd_comb(concl(th2));
-
+  state = consequent(conclusion(th2));
+  
   thm entail = spec(snd_binop(parse_term("hsep"), state), mp(get_theorem("hsep_cancel_right"), th));
   entail = sep_normalize_rule(entail);
-  thm th_pre_norm = sep_cancel(state, fst_binop(parse_term("hentail"), concl(entail)));
+
+  
+  thm th_pre_norm = sep_cancel(old_state, fst_binop(parse_term("hentail"), conclusion(entail)));
   entail = once_rewrite_rule(th_pre_norm, entail);
 
   // Construct `hexists` with binders (in order) in `exists_list`.
@@ -183,3 +211,48 @@ thm which_implies(term state, thm th) {
   return entail;
 }
 
+// [[cstar::function(
+// thm hfact_auto(term pres[], term posts[]) {
+//   thm result = spec(`emp`, get_theorem("hentail_refl")); // emp |-- emp
+//   term pre_conj = `T`;
+// 
+//   int i = 0;
+//   while (1) {
+//     if (pres[i] == NULL) break;
+//     term pre = pres[i];
+//     pre_conj = `(${pre_conj:bool}) /\ (${pre:bool})`;
+//     i = i + 1;
+//   }
+// 
+//   i = 0;
+//   while (1) {
+//     if (posts[i] == NULL) break;
+//     term post = posts[i];
+//     term check_post_i = `${pre_conj:bool} ==> ${post:bool}`;
+//     thm arith = arith_rule(check_post_i);
+//     if (equals_term(conclusion(arith), check_post_i)) {
+//       result = mp(mp(get_theorem("hfact_intro"), mp(arith, assume(pre_conj))), result);
+//     }
+//     i = i + 1;
+//   }
+// 
+//   puts("hfact_auto");
+//   puts(string_of_thm(result));
+// 
+//   i = 0;
+//   while (1) {
+//     if (pres[i] == NULL) break;
+//     int j = 0;
+//     while (1) {
+//       if (posts[j] == NULL) break;
+//       if (equals_term(pres[i], posts[j])) {
+// 
+//       }
+//       j = j + 1;
+//     }
+//     i = i + 1;
+//   }
+// 
+//   return sep_normalize_rule(result);
+// }
+// )]];
